tryrecv wip, edit network state

lang.v
@@ -238,7 +238,7 @@ Proof. refine (inj_countable of_val to_val _); auto using to_of_val. Qed.
 
 
 Record state : Type := {
-  chan: gmap loc (option (gset val));
+  chan: gmap loc (gset val);
 }.
 Global Instance state_inhabited : Inhabited state :=
   populate {|
@@ -309,7 +309,7 @@ Definition subst' (mx : binder) (v : val) : expr → expr :=
   match mx with BNamed x => subst x v | BAnon => id end.
 
 (** The stepping relation *)
-Definition state_upd_chan (f: gmap loc (option (gset val)) → gmap loc (option (gset val))) (σ: state) : state :=
+Definition state_upd_chan (f: gmap loc (gset val) → gmap loc (gset val)) (σ: state) : state :=
   {| chan := f σ.(chan)|}.
 Global Arguments state_upd_chan !_ /.
 
@@ -383,23 +383,23 @@ Inductive head_step : expr → state → list observation → expr → state →
       σ.(chan) !! c = None ->
       head_step NewCh σ
                 []
-                (Val $ LitV $ LitLoc c) (state_upd_chan <[c := Some $ empty]> σ)
+                (Val $ LitV $ LitLoc c) (state_upd_chan <[c := empty]> σ)
                 []
   | SendS σ M c v:
-      σ.(chan) !! c = Some $ Some $ M ->
+      σ.(chan) !! c = Some $ M ->
       head_step (Send (Val $ LitV $ LitLoc c) (Val v)) σ
                 []
-                (Val $ LitV LitUnit) (state_upd_chan <[c := Some $ M ∪ {[ v ]}]> σ)
+                (Val $ LitV LitUnit) (state_upd_chan <[c := M ∪ {[ v ]}]> σ)
                 []
   | TryRecvNoneS σ c:
-      σ.(chan) !! c = Some $ Some $ empty ->
+      σ.(chan) !! c = Some $ empty ->
       head_step (TryRecv (Val $ LitV $ LitLoc c)) σ
                 [] None_ σ []
   | TryRecvSomeS σ c M v:
-      σ.(chan) !! c = Some $ Some $ (M ∪ {[ v ]}) ->
+      σ.(chan) !! c = Some $ (M ∪ {[ v ]}) ->
       head_step (TryRecv (Val $ LitV $ LitLoc c)) σ
                 []
-                (Some_ v) (state_upd_chan <[c := Some M]> σ)
+                (Some_ v) (state_upd_chan <[c := M]> σ)
                 [].
 
 (** Basic properties about the language *)
@@ -476,7 +476,7 @@ Proof. destruct 1; inversion 1; naive_solver. Qed.
 Lemma alloc_newch σ :
   let l := fresh_locs (dom (gset _) σ.(chan)) +ₗ 0 in
   head_step NewCh σ []
-            (Val $ LitV $ LitLoc l) (state_upd_chan <[l := Some ∅]> σ) [].
+            (Val $ LitV $ LitLoc l) (state_upd_chan <[l := ∅]> σ) [].
 Proof.
   intros.
   eapply NewChS.
